Simplified session channel, and proved send spec up to laters

new/proof/github_com/goose_lang/goose/model/channel/protocol/dsp/dsp.v
@@ -9,16 +9,14 @@ From New.proof.github_com.goose_lang.goose.model.channel
     This file implements dependent separation protocols using bidirectional Go channels.
 
     Key concepts:
-    - Two protocol endpoints (left and right) communicate via two Go channels
-    - LR channel: left endpoint sends V_LR values to right endpoint
-    - RL channel: right endpoint sends V_RL values to left endpoint
+    - Protocol endpoints communicate via two Go channels
+    - LR channel: left endpoint sends values to right endpoint
+    - RL channel: right endpoint sends values to left endpoint
     - Protocol state is tracked using Actris iProto with sum types
     - Channel closure is protocol-aware - only allowed when protocol permits
 *)
 
 (** ** Sum Type for Bidirectional Communication *)
-
-Definition DspV (V_LR V_RL : Type) := sum V_LR V_RL.
 
 #[export] Instance eqdec_sum `{EqDecision A} `{EqDecision B}
   : EqDecision (A + B) := _.
@@ -28,8 +26,15 @@ Definition DspV (V_LR V_RL : Type) := sum V_LR V_RL.
 Section dsp.
 Context `{hG: heapGS Σ, !ffi_semantics _ _}.
 Context `{!ghost_varG Σ ()}.
-Context `{!chanGhostStateG Σ ()}.
+Context `{!chanGhostStateG Σ val}.
 Context `{!globalsGS Σ} {go_ctx : GoContext}.
+Context `{!protoG Σ val}.
+
+#[export] Instance into_val_val : IntoVal val := { to_val_def := id }.
+Instance into_val_typed_val : IntoValTyped val atomic.Value.
+Proof. Admitted.
+
+Let N := nroot .@ "dsp_chan".
 
 (** ** Buffer Matching Predicates *)
 
@@ -43,31 +48,18 @@ Definition buffer_matches {V}
   | _ => vs = []
   end.
 
-(** ** Protocol Value Lifting *)
-
-(** Lift left-to-right values into sum type for protocol *)
-Definition lift_lr {V_LR V_RL} (vsl : list V_LR)
-  : list (DspV V_LR V_RL) := List.map (@inl V_LR V_RL) vsl.
-
-(** Lift right-to-left values into sum type for protocol *)
-Definition lift_rl {V_LR V_RL} (vsr : list V_RL)
-  : list (DspV V_LR V_RL) := List.map (@inr V_LR V_RL) vsr.
-
 (** ** DSP Session Context *)
 
 (** DSP session invariant - owns both channels and maintains protocol state *)
-Definition dsp_session_inv {V_LR V_RL}
-    `{!protoG Σ (DspV V_LR V_RL)}
-    `{!chanGhostStateG Σ V_LR} `{!IntoVal V_LR} `{!IntoValTyped V_LR tL}
-    `{!chanGhostStateG Σ V_RL} `{!IntoVal V_RL} `{!IntoValTyped V_RL tR}
+Definition dsp_session_inv
     (γl γr : gname)
     (lr_chan rl_chan : loc) (γlr_names γrl_names : chan_names)
     (lrcap rlcap: Z) : iProp Σ :=
   ∃ lr_state rl_state vsl vsr,
-    own_channel lr_chan lrcap lr_state γlr_names ∗
-    own_channel rl_chan rlcap rl_state γrl_names ∗
     ⌜buffer_matches lr_state vsl⌝ ∗
     ⌜buffer_matches rl_state vsr⌝ ∗
+    own_channel lr_chan lrcap lr_state γlr_names ∗
+    own_channel rl_chan rlcap rl_state γrl_names ∗
     match lr_state with
     | chan_rep.Closed _ => iProto_own γl END
     | _ => True
@@ -76,14 +68,21 @@ Definition dsp_session_inv {V_LR V_RL}
     | chan_rep.Closed _ => iProto_own γr END
     | _ => True
     end ∗
-    iProto_ctx γl γr (lift_lr vsl) (lift_rl vsr).
+    iProto_ctx γl γr vsl vsr.
+
+Lemma dsp_session_inv_sym
+    γl γr lr_chan rl_chan γlr_names γrl_names lrcap rlcap :
+   dsp_session_inv γl γr lr_chan rl_chan γlr_names γrl_names lrcap rlcap ⊣⊢
+   dsp_session_inv γr γl rl_chan lr_chan γrl_names γlr_names rlcap lrcap.
+Proof.
+  iSplit.
+  - iDestruct 1 as (????) "(Hcl&Hcr&?&?&?&?&Hp)". iFrame. by iApply iProto_ctx_sym.
+  - iDestruct 1 as (????) "(Hcl&Hcr&?&?&?&?&Hp)". iFrame. by iApply iProto_ctx_sym.
+Qed.
 
 (** DSP session context - public interface with persistent channel handles *)
-Definition dsp_session {V_LR V_RL}
-    `{!protoG Σ (DspV V_LR V_RL)}
-    `{!chanGhostStateG Σ V_LR} `{!IntoVal V_LR} `{!IntoValTyped V_LR tL}
-    `{!chanGhostStateG Σ V_RL} `{!IntoVal V_RL} `{!IntoValTyped V_RL tR}
-    (γl γr : gname) (N : namespace)
+Definition dsp_session
+    (γl γr : gname)
     (lr_chan rl_chan : loc) (γlr_names γrl_names : chan_names)
     (lrcap rlcap: Z) : iProp Σ :=
   is_channel lr_chan lrcap γlr_names ∗
@@ -93,192 +92,136 @@ Definition dsp_session {V_LR V_RL}
 (** ** DSP Endpoints *)
 
 (** Left endpoint - can send V_LR via lr_chan, receive V_RL via rl_chan *)
-Definition dsp_left_endpoint {V_LR V_RL}
-    `{!protoG Σ (DspV V_LR V_RL)}
-    `{!chanGhostStateG Σ V_LR} `{!IntoVal V_LR} `{!IntoValTyped V_LR tL}
-    `{!chanGhostStateG Σ V_RL} `{!IntoVal V_RL} `{!IntoValTyped V_RL tR}
-    (γl γr : gname) (N : namespace)
-    (lr_chan rl_chan : loc) (γlr_names γrl_names : chan_names)
-    (lrcap rlcap: Z)
-    (p : option $ iProto Σ (DspV V_LR V_RL)) : iProp Σ :=
-  dsp_session γl γr N lr_chan rl_chan γlr_names γrl_names lrcap rlcap ∗
-  match p with
-  | None => True
-  | Some p => iProto_own γl p
-  end.
+Definition dsp_endpoint
+    (v:val)
+    (p : option $ iProto Σ val) : iProp Σ :=
+  ∃ (γl γr : gname) (lr_chan rl_chan : loc) (γlr_names γrl_names : chan_names)
+    (lrcap rlcap: Z),
+    ⌜v = #lr_chan⌝ ∗
+    dsp_session γl γr lr_chan rl_chan γlr_names γrl_names lrcap rlcap ∗
+    match p with
+    | None => True
+    | Some p => iProto_own γl p
+    end.
 
-(** Right endpoint - can send V_RL via rl_chan, receive V_LR via lr_chan *)
-Definition dsp_right_endpoint {V_LR V_RL}
-    `{!protoG Σ (DspV V_LR V_RL)}
-    `{!chanGhostStateG Σ V_LR} `{!IntoVal V_LR} `{!IntoValTyped V_LR tL}
-    `{!chanGhostStateG Σ V_RL} `{!IntoVal V_RL} `{!IntoValTyped V_RL tR}
-    (γl γr : gname) (N : namespace)
-    (lr_chan rl_chan : loc) (γlr_names γrl_names : chan_names)
-    (lrcap rlcap: Z)
-    (p : option $ iProto Σ (DspV V_LR V_RL)) : iProp Σ :=
-  dsp_session γl γr N lr_chan rl_chan γlr_names γrl_names lrcap rlcap ∗
-  match p with
-  | None => True
-  | Some p => iProto_own γr p
-  end.
+Notation "c ↣ p" := (dsp_endpoint c (Some p)) (at level 20, format "c  ↣  p").
+Notation "↯ c" := (dsp_endpoint c None) (at level 20, format "↯  c").
 
 (** ** Initialization *)
 
 (** Initialize a new DSP session from basic channels *)
-Lemma dsp_session_init {V_LR V_RL}
-    `{!protoG Σ (DspV V_LR V_RL)}
-    `{cGSL : chanGhostStateG Σ V_LR} `{!IntoVal V_LR} `{!IntoValTyped V_LR tL}
-    `{cGSR : chanGhostStateG Σ V_RL} `{!IntoVal V_RL} `{!IntoValTyped V_RL tR}
-    E
-    (N : namespace) (lr_chan rl_chan : loc) (γlr_names γrl_names : chan_names)
-    (lrcap rlcap: Z) (p : iProto Σ (DspV V_LR V_RL)) :
+Lemma dsp_session_init
+    E (lr_chan rl_chan : loc) (γlr_names γrl_names : chan_names)
+    (lrcap rlcap: Z) (p : iProto Σ val) :
   is_channel lr_chan lrcap γlr_names -∗
   is_channel rl_chan rlcap γrl_names -∗
-  @own_channel _ _ cGSL lr_chan lrcap chan_rep.Idle γlr_names -∗
-  @own_channel _ _ cGSR rl_chan rlcap chan_rep.Idle γrl_names ={E}=∗
-  ∃ γl γr,
-    dsp_left_endpoint γl γr N lr_chan rl_chan γlr_names γrl_names lrcap rlcap (Some p) ∗
-    dsp_right_endpoint γl γr N lr_chan rl_chan γlr_names γrl_names lrcap rlcap (Some $ iProto_dual p).
+  own_channel lr_chan lrcap chan_rep.Idle γlr_names -∗
+  own_channel rl_chan rlcap chan_rep.Idle γrl_names ={E}=∗
+  #lr_chan ↣ p ∗ #rl_chan ↣ iProto_dual p.
 Proof.
   iIntros "#Hcl_is #Hcr_is Hcl_own Hcr_own".
   iMod (iProto_init) as (γl γr) "(Hctx & Hpl & Hpr)".
-  iMod (inv_alloc N _ (dsp_session_inv _ _ _ _ _ _ _ _) with "[Hcl_own Hcr_own Hctx]")
+  iMod (inv_alloc N _ (dsp_session_inv γl γr lr_chan rl_chan γlr_names γrl_names lrcap rlcap) with "[Hcl_own Hcr_own Hctx]")
     as "#Hinv".
   { iExists chan_rep.Idle,chan_rep.Idle,[],[]. by iFrame. }
-  by iFrame "∗#".
+  iModIntro.
+  iSplitL "Hpl".
+  - iExists _,_,_,_,_,_,_,_. iSplit; [done|].    
+    iFrame "Hpl Hinv". iFrame "∗#".
+  - iExists _,_,_,_,_,_,_,_. iSplit; [done|].
+    rewrite dsp_session_inv_sym. iFrame "Hinv".
+    iFrame "∗#".
 Qed.
 
-(** ** Left Endpoint Operations *)
+(** ** Endpoint Operations *)
 
-(** Left endpoint sends V_LR value via lr_chan *)
-Lemma dsp_left_send {V_LR V_RL}
-    `{!protoG Σ (DspV V_LR V_RL)}
-    `{!chanGhostStateG Σ V_LR} `{!IntoVal V_LR} `{!IntoValTyped V_LR tL}
-    `{!chanGhostStateG Σ V_RL} `{!IntoVal V_RL} `{!IntoValTyped V_RL tR}
-    (γl γr : gname) (N : namespace)
-    (lr_chan rl_chan : loc) (γlr_names γrl_names : chan_names)
-    (lrcap rlcap: Z) (v : V_LR) (p : iProto Σ (DspV V_LR V_RL)) :
-  {{{ is_pkg_init channel ∗
-      dsp_left_endpoint γl γr N lr_chan rl_chan γlr_names γrl_names lrcap rlcap (Some $ <!> MSG (inl v); p) }}}
-    lr_chan @ (ptrT.id channel.Channel.id) @ "Send" #tL #v
-  {{{ RET #();
-      dsp_left_endpoint γl γr N lr_chan rl_chan γlr_names γrl_names lrcap rlcap (Some p) }}}.
+Lemma into_val_val_unfold (v : val) : #v = v.
+Proof. by rewrite to_val_unseal /to_val_def /=. Qed.
+
+(** Endpoint sends value *)
+Lemma dsp_send (c : val) (v : val) (p : iProto Σ val) :
+  {{{ is_pkg_init channel ∗ c ↣ <!> MSG v; p }}}
+    c @ (ptrT.id channel.Channel.id) @ "Send" #atomic.Value #v
+  {{{ RET #(); c ↣ p }}}.
+Proof.
+  iIntros (Φ) "(#Hinit&Hc) HΦ".
+  iDestruct "Hc" as (????????->) "(#(Hcl&Hcr&HI)&Hp)".
+  replace (# (# lr_chan)) with (# lr_chan); last first.
+  { by rewrite into_val_val_unfold. }
+  iApply (wp_Send lr_chan lrcap v γlr_names with "[$Hinit $Hcl]").
+  iIntros "H£".
+  iMod (inv_acc with "HI") as "[IH Hclose]"; [solve_ndisj|].
+  iDestruct "IH" as (????) "(>%&>%&Hownl&Hownr&Hclosel&Hcloser&Hctx)".
+  iApply fupd_mask_intro; [solve_ndisj|]. 
+  iIntros "Hclose'".
+  iModIntro.
+  iExists _. iFrame.
+  destruct lr_state.
+  - destruct (length buff <? lrcap)%Z; [|done].
+    iIntros "Hownl".
+    iDestruct (iProto_send _ _ _ _ _ v p with "Hctx [$Hp] []") as "Hp".
+    { by rewrite iMsg_base_eq. }
+    iMod "Hp" as "[Hp Hown]". iMod "Hclose'" as "_".
+    iMod ("Hclose" with "[Hownl Hownr Hclosel Hcloser Hp]").
+    { iIntros "!>". iExists _,_,_,_. iFrame. do 2 (iSplit; [done|]).
+      iFrame. inversion H. subst. admit. }    
+    iApply "HΦ". by iFrame "#∗".
+  - iIntros "Hownl".
+    iDestruct (iProto_send _ _ _ _ _ v p with "Hctx [$Hp] []") as "Hp".
+    { by rewrite iMsg_base_eq. }
+    iMod "Hp" as "[Hctx Hown]". iMod "Hclose'" as "_". 
+    iMod ("Hclose" with "[Hownl Hownr Hclosel Hcloser Hctx]").
+    { iIntros "!>". iExists _,_,_,_. iFrame. do 2 (iSplit; [done|]).
+      iFrame. inversion H. subst. admit. }
+    iModIntro.
+    iMod (inv_acc with "HI") as "[IH Hclose]"; [solve_ndisj|].
+    iApply fupd_mask_intro; [solve_ndisj|]. iIntros "Hclose'".
+    iDestruct "IH" as (????) "(>%&>%&Hownl&Hownr&Hclosel&Hcloser&Hctx)".
+    iFrame.
+    iIntros "!>".
+    destruct lr_state; try done.
+    + iIntros "Hownl". iMod "Hclose'".
+      iMod ("Hclose" with "[Hownl Hownr Hclosel Hcloser Hctx]").
+      { iIntros "!>". iExists _,_,_,_. iFrame. done. }
+      iApply "HΦ". iFrame "#∗". done.
+    + iDestruct (iProto_own_excl with "Hown Hclosel") as "[]".
+  - done.
+  - iIntros "Hownl".
+    iDestruct (iProto_send _ _ _ _ _ v p with "Hctx [$Hp] []") as "Hp".
+    { by rewrite iMsg_base_eq. }
+    iMod "Hp" as "[Hp Hown]". iMod "Hclose'".
+    iMod ("Hclose" with "[Hownl Hownr Hclosel Hcloser Hp]").
+    { iIntros "!>". iExists _,_,_,_. iFrame. do 2 (iSplit; [done|]).
+      iFrame. inversion H. subst. admit. }
+    iApply "HΦ". by iFrame "#∗".
+  - done.
+  - done.
+  - iDestruct (iProto_own_excl with "Hp Hclosel") as "[]".
+Admitted.
+
+(** Endpoint receives value *)
+Lemma dsp_recv {TT:tele}
+    (c: val) (v : TT → val) (P : TT → iProp Σ) (p : TT → iProto Σ val) :
+  {{{ is_pkg_init channel ∗ c ↣ <?.. x> MSG (v x) {{ ▷ P x }}; p x }}}
+    c @ (ptrT.id channel.Channel.id) @ "Receive" #atomic.Value #()
+  {{{ x, RET (#(v x), #true); c ↣ p x ∗ P x }}}.
 Proof.
 Admitted.
 
-(** Left endpoint receives V_RL value via rl_chan *)
-Lemma dsp_left_recv {TT:tele} {V_LR V_RL}
-    `{!protoG Σ (DspV V_LR V_RL)}
-    `{!chanGhostStateG Σ V_LR} `{!IntoVal V_LR} `{!IntoValTyped V_LR tL}
-    `{!chanGhostStateG Σ V_RL} `{!IntoVal V_RL} `{!IntoValTyped V_RL tR}
-    (γl γr : gname) (N : namespace)
-    (lr_chan rl_chan : loc) (γlr_names γrl_names : chan_names)
-    (lrcap rlcap: Z) (v : TT → V_LR) (P : TT → iProp Σ) (p : TT → iProto Σ (DspV V_LR V_RL)) :
-  {{{ is_pkg_init channel ∗
-      dsp_left_endpoint γl γr N lr_chan rl_chan γlr_names γrl_names lrcap rlcap
-        (Some $ <?.. x> MSG inl (v x) {{ ▷ P x }}; p x) }}}
-    rl_chan @ (ptrT.id channel.Channel.id) @ "Receive" #tR #()
-  {{{ x, RET (#(v x), #true);
-      dsp_left_endpoint γl γr N lr_chan rl_chan γlr_names γrl_names lrcap rlcap (Some $ p x) ∗
-      P x }}}.
-Proof.
-Admitted.
-
-Lemma dsp_left_recv_closed {TT:tele} {V_LR V_RL}
-    `{!protoG Σ (DspV V_LR V_RL)}
-    `{!chanGhostStateG Σ V_LR} `{!IntoVal V_LR} `{!IntoValTyped V_LR tL}
-    `{!chanGhostStateG Σ V_RL} `{!IntoVal V_RL} `{!IntoValTyped V_RL tR}
-    (γl γr : gname) (N : namespace)
-    (lr_chan rl_chan : loc) (γlr_names γrl_names : chan_names)
-    (lrcap rlcap: Z) p :
-  p = Some END ∨ p = None →
-  {{{ is_pkg_init channel ∗
-      dsp_left_endpoint γl γr N lr_chan rl_chan γlr_names γrl_names lrcap rlcap p }}}
-    rl_chan @ (ptrT.id channel.Channel.id) @ "Receive" #tR #()
+(** Endpoint receives on a closed or ended channel *)
+Lemma dsp_recv_closed {TT:tele} (c : val) :
+  {{{ is_pkg_init channel ∗ (c ↣ END ∨ ↯ c) }}}
+    c @ (ptrT.id channel.Channel.id) @ "Receive" #atomic.Value #()
   {{{ RET (#(), #false);
-      dsp_left_endpoint γl γr N lr_chan rl_chan γlr_names γrl_names lrcap rlcap p }}}.
+      dsp_endpoint c None }}}.
 Proof.
 Admitted.
 
-(** Left endpoint closes lr_chan (stops sending V_LR) *)
-Lemma dsp_left_close_lr {V_LR V_RL}
-    `{!protoG Σ (DspV V_LR V_RL)}
-    `{!chanGhostStateG Σ V_LR} `{!IntoVal V_LR} `{!IntoValTyped V_LR tL}
-    `{!chanGhostStateG Σ V_RL} `{!IntoVal V_RL} `{!IntoValTyped V_RL tR}
-    (γl γr : gname) (N : namespace)
-    (lr_chan rl_chan : loc) (γlr_names γrl_names : chan_names)
-    (lrcap rlcap: Z) (p : iProto Σ (DspV V_LR V_RL)) :
-  {{{ is_pkg_init channel ∗
-      dsp_left_endpoint γl γr N lr_chan rl_chan γlr_names γrl_names lrcap rlcap (Some END) }}}
-    lr_chan @ (ptrT.id channel.Channel.id) @ "Close" #tL #()
-  {{{ RET #(); dsp_left_endpoint γl γr N lr_chan rl_chan γlr_names γrl_names lrcap rlcap None }}}.
-Proof.
-Admitted.
-
-(** ** Right Endpoint Operations *)
-
-(** Right endpoint sends V_RL value via rl_chan *)
-Lemma dsp_right_send {V_LR V_RL}
-    `{!protoG Σ (DspV V_LR V_RL)}
-    `{!chanGhostStateG Σ V_LR} `{!IntoVal V_LR} `{!IntoValTyped V_LR tL}
-    `{!chanGhostStateG Σ V_RL} `{!IntoVal V_RL} `{!IntoValTyped V_RL tR}
-    (γl γr : gname) (N : namespace)
-    (lr_chan rl_chan : loc) (γlr_names γrl_names : chan_names)
-    (lrcap rlcap: Z) (v : V_RL) (p : iProto Σ (DspV V_LR V_RL)) :
-  {{{ is_pkg_init channel ∗
-      dsp_right_endpoint γl γr N lr_chan rl_chan γlr_names γrl_names lrcap rlcap (Some $ <!> MSG (inr v); p) }}}
-    rl_chan @ (ptrT.id channel.Channel.id) @ "Send" #tR #v
-  {{{ RET #();
-      dsp_right_endpoint γl γr N lr_chan rl_chan γlr_names γrl_names lrcap rlcap (Some p) }}}.
-Proof.
-Admitted.
-
-(** Right endpoint receives V_LR value via lr_chan *)
-Lemma dsp_right_recv {TT:tele} {V_LR V_RL}
-    `{!protoG Σ (DspV V_LR V_RL)}
-    `{!chanGhostStateG Σ V_LR} `{!IntoVal V_LR} `{!IntoValTyped V_LR tL}
-    `{!chanGhostStateG Σ V_RL} `{!IntoVal V_RL} `{!IntoValTyped V_RL tR}
-    (γl γr : gname) (N : namespace)
-    (lr_chan rl_chan : loc) (γlr_names γrl_names : chan_names)
-    (lrcap rlcap: Z) (v : TT → V_RL) (P : TT → iProp Σ) (p : TT → iProto Σ (DspV V_LR V_RL)) :
-  {{{ is_pkg_init channel ∗
-      dsp_right_endpoint γl γr N lr_chan rl_chan γlr_names γrl_names lrcap rlcap
-        (Some $ <?.. x> MSG inr (v x) {{ ▷ P x }}; p x) }}}
-    lr_chan @ (ptrT.id channel.Channel.id) @ "Receive" #tL #()
-  {{{ x, RET (#(v x), #true);
-      dsp_right_endpoint γl γr N lr_chan rl_chan γlr_names γrl_names lrcap rlcap (Some $ p x) ∗
-      P x }}}.
-Proof.
-Admitted.
-
-Lemma dsp_right_recv_closed {TT:tele} {V_LR V_RL}
-    `{!protoG Σ (DspV V_LR V_RL)}
-    `{!chanGhostStateG Σ V_LR} `{!IntoVal V_LR} `{!IntoValTyped V_LR tL}
-    `{!chanGhostStateG Σ V_RL} `{!IntoVal V_RL} `{!IntoValTyped V_RL tR}
-    (γl γr : gname) (N : namespace)
-    (lr_chan rl_chan : loc) (γlr_names γrl_names : chan_names)
-    (lrcap rlcap: Z) p :
-  p = Some END ∨ p = None →
-  {{{ is_pkg_init channel ∗
-      dsp_right_endpoint γl γr N lr_chan rl_chan γlr_names γrl_names lrcap rlcap p }}}
-    rl_chan @ (ptrT.id channel.Channel.id) @ "Receive" #tR #()
-  {{{ RET (#(), #false);
-      dsp_right_endpoint γl γr N lr_chan rl_chan γlr_names γrl_names lrcap rlcap p }}}.
-Proof.
-Admitted.
-
-(** Right endpoint closes rl_chan (stops sending V_RL) *)
-Lemma dsp_right_close_rl {V_LR V_RL}
-    `{!protoG Σ (DspV V_LR V_RL)}
-    `{!chanGhostStateG Σ V_LR} `{!IntoVal V_LR} `{!IntoValTyped V_LR tL}
-    `{!chanGhostStateG Σ V_RL} `{!IntoVal V_RL} `{!IntoValTyped V_RL tR}
-    (γl γr : gname) (N : namespace)
-    (lr_chan rl_chan : loc) (γlr_names γrl_names : chan_names)
-    (lrcap rlcap: Z) (p : iProto Σ (DspV V_LR V_RL)) :
-  {{{ is_pkg_init channel ∗
-      dsp_right_endpoint γl γr N lr_chan rl_chan γlr_names γrl_names lrcap rlcap (Some END) }}}
-    rl_chan @ (ptrT.id channel.Channel.id) @ "Close" #tR #()
-  {{{ RET #(); dsp_right_endpoint γl γr N lr_chan rl_chan γlr_names γrl_names lrcap rlcap None }}}.
+(** Endpoint closes (stops sending val) *)
+Lemma dsp_close  (c : val) (p : iProto Σ val) :
+  {{{ is_pkg_init channel ∗ c ↣ END }}}
+    c @ (ptrT.id channel.Channel.id) @ "Close" #atomic.Value #()
+  {{{ RET #(); ↯ c }}}.
 Proof.
 Admitted.
 
